Norm not finished

softwarefoundations/vol2_plf/Norm.v
@@ -5,3 +5,936 @@ From PLF Require Import Maps.
 From PLF Require Import Smallstep.
 
 Hint Constructors multi : core.
+
+Inductive ty : Type :=
+  | Ty_Bool : ty
+  | Ty_Arrow : ty -> ty -> ty
+  | Ty_Prod : ty -> ty -> ty.
+
+Inductive tm : Type :=
+    (* pure STLC *)
+  | tm_var : string -> tm
+  | tm_app : tm -> tm -> tm
+  | tm_abs : string -> ty -> tm -> tm
+    (* booleans *)
+  | tm_true : tm
+  | tm_false : tm
+  | tm_if : tm -> tm -> tm -> tm
+    (* pairs *)
+  | tm_pair : tm -> tm -> tm
+  | tm_fst : tm -> tm
+  | tm_snd : tm -> tm.
+
+Declare Custom Entry stlc.
+Notation "<{ e }>" := e (e custom stlc at level 99).
+Notation "( x )" := x (in custom stlc, x at level 99).
+Notation "x" := x (in custom stlc at level 0, x constr at level 0).
+Notation "S -> T" := (Ty_Arrow S T) (in custom stlc at level 50, right associativity).
+Notation "x y" := (tm_app x y) (in custom stlc at level 1, left associativity).
+Notation "\ x : t , y" := (tm_abs x t y) (in custom stlc at level 90, x at level 99,
+                           t custom stlc at level 99,
+                           y custom stlc at level 99,
+                           left associativity).
+Coercion tm_var : string >-> tm.
+Notation "{ x }" := x (in custom stlc at level 1, x constr).
+Notation "'Bool'" := Ty_Bool (in custom stlc at level 0).
+Notation "'if' x 'then' y 'else' z" := (tm_if x y z) (in custom stlc at level 89,
+                                        x custom stlc at level 99,
+                                        y custom stlc at level 99,
+                                        z custom stlc at level 99,
+                                        left associativity).
+Notation "'true'" := true (at level 1).
+Notation "'true'" := tm_true (in custom stlc at level 0).
+Notation "'false'" := false (at level 1).
+Notation "'false'" := tm_false (in custom stlc at level 0).
+Notation "X * Y" := (Ty_Prod X Y) (in custom stlc at level 2, X custom stlc, Y custom stlc at level 0).
+Notation "( x ',' y )" := (tm_pair x y) (in custom stlc at level 0,
+                                                x custom stlc at level 99,
+                                                y custom stlc at level 99).
+Notation "t '.fst'" := (tm_fst t) (in custom stlc at level 0).
+Notation "t '.snd'" := (tm_snd t) (in custom stlc at level 0).
+
+
+
+
+Reserved Notation "'[' x ':=' s ']' t" (in custom stlc at level 20, x constr).
+Fixpoint subst (x : string) (s : tm) (t : tm) : tm :=
+  match t with
+  | tm_var y =>
+      if eqb_string x y then s else t
+  | <{ \ y : T, t1 }> =>
+      if eqb_string x y then t else <{ \y:T, [x:=s] t1 }>
+  | <{t1 t2}> =>
+      <{ ([x:=s]t1) ([x:=s]t2)}>
+  | <{true}> =>
+      <{true}>
+  | <{false}> =>
+      <{false}>
+  | <{if t1 then t2 else t3}> =>
+      <{if ([x:=s] t1) then ([x:=s] t2) else ([x:=s] t3)}>
+  | <{(t1, t2)}> =>
+      <{( ([x:=s] t1), ([x:=s] t2) )}>
+  | <{t0.fst}> =>
+      <{ ([x:=s] t0).fst}>
+  | <{t0.snd}> =>
+      <{ ([x:=s] t0).snd}>
+  end
+where "'[' x ':=' s ']' t" := (subst x s t) (in custom stlc).
+
+
+Inductive value : tm -> Prop :=
+  | v_abs : forall x T2 t1,
+      value <{\x:T2, t1}>
+  | v_true :
+      value <{true}>
+  | v_false :
+      value <{false}>
+  | v_pair : forall v1 v2,
+      value v1 ->
+      value v2 ->
+      value <{(v1, v2)}>.
+Hint Constructors value : core.
+
+
+Reserved Notation "t '-->' t'" (at level 40).
+Inductive step : tm -> tm -> Prop :=
+  | ST_AppAbs : forall x T2 t1 v2,
+         value v2 ->
+         <{(\x:T2, t1) v2}> --> <{ [x:=v2]t1 }>
+  | ST_App1 : forall t1 t1' t2,
+         t1 --> t1' ->
+         <{t1 t2}> --> <{t1' t2}>
+  | ST_App2 : forall v1 t2 t2',
+         value v1 ->
+         t2 --> t2' ->
+         <{v1 t2}> --> <{v1 t2'}>
+  | ST_IfTrue : forall t1 t2,
+      <{if true then t1 else t2}> --> t1
+  | ST_IfFalse : forall t1 t2,
+      <{if false then t1 else t2}> --> t2
+  | ST_If : forall t1 t1' t2 t3,
+      t1 --> t1' ->
+      <{if t1 then t2 else t3}> --> <{if t1' then t2 else t3}>
+  | ST_Pair1 : forall t1 t1' t2,
+        t1 --> t1' ->
+        <{ (t1,t2) }> --> <{ (t1' , t2) }>
+  | ST_Pair2 : forall v1 t2 t2',
+        value v1 ->
+        t2 --> t2' ->
+        <{ (v1, t2) }> --> <{ (v1, t2') }>
+  | ST_Fst1 : forall t0 t0',
+        t0 --> t0' ->
+        <{ t0.fst }> --> <{ t0'.fst }>
+  | ST_FstPair : forall v1 v2,
+        value v1 ->
+        value v2 ->
+        <{ (v1,v2).fst }> --> v1
+  | ST_Snd1 : forall t0 t0',
+        t0 --> t0' ->
+        <{ t0.snd }> --> <{ t0'.snd }>
+  | ST_SndPair : forall v1 v2,
+        value v1 ->
+        value v2 ->
+        <{ (v1,v2).snd }> --> v2
+where "t '-->' t'" := (step t t').
+Hint Constructors step : core.
+
+Notation multistep := (multi step).
+Notation "t1 '-->*' t2" := (multistep t1 t2) (at level 40).
+
+Notation step_normal_form := (normal_form step).
+
+Lemma value__normal : forall t, value t -> step_normal_form t.
+Proof with eauto.
+  intros t H; induction H; intros [t' ST]; inversion ST...
+Qed.
+
+
+Definition context := partial_map ty.
+
+Reserved Notation "Gamma '|-' t '\in' T" (at level 40, t custom stlc, T custom stlc at level 0).
+Inductive has_type : context -> tm -> ty -> Prop :=
+  | T_Var : forall Gamma x T1,
+      Gamma x = Some T1 ->
+      Gamma |- x \in T1
+  | T_Abs : forall Gamma x T1 T2 t1,
+    (x |-> T2 ; Gamma) |- t1 \in T1 ->
+      Gamma |- \x:T2, t1 \in (T2 -> T1)
+  | T_App : forall T1 T2 Gamma t1 t2,
+      Gamma |- t1 \in (T2 -> T1) ->
+      Gamma |- t2 \in T2 ->
+      Gamma |- t1 t2 \in T1
+  | T_True : forall Gamma,
+       Gamma |- true \in Bool
+  | T_False : forall Gamma,
+       Gamma |- false \in Bool
+  | T_If : forall t1 t2 t3 T1 Gamma,
+       Gamma |- t1 \in Bool ->
+       Gamma |- t2 \in T1 ->
+       Gamma |- t3 \in T1 ->
+       Gamma |- if t1 then t2 else t3 \in T1
+  | T_Pair : forall Gamma t1 t2 T1 T2,
+      Gamma |- t1 \in T1 ->
+      Gamma |- t2 \in T2 ->
+      Gamma |- (t1, t2) \in (T1 * T2)
+  | T_Fst : forall Gamma t0 T1 T2,
+      Gamma |- t0 \in (T1 * T2) ->
+      Gamma |- t0.fst \in T1
+  | T_Snd : forall Gamma t0 T1 T2,
+      Gamma |- t0 \in (T1 * T2) ->
+      Gamma |- t0.snd \in T2
+where "Gamma '|-' t '\in' T" := (has_type Gamma t T).
+Hint Constructors has_type : core.
+
+Hint Extern 2 (has_type _ (app _ _) _) => eapply T_App; auto : core.
+Hint Extern 2 (_ = _) => compute; reflexivity : core.
+
+Lemma weakening : forall Gamma Gamma' t T,
+     inclusion Gamma Gamma' ->
+     Gamma  |- t \in T ->
+     Gamma' |- t \in T.
+Proof.
+  intros Gamma Gamma' t T H Ht.
+  generalize dependent Gamma'.
+  induction Ht; eauto using inclusion_update.
+Qed.
+
+Lemma weakening_empty : forall Gamma t T,
+     empty |- t \in T ->
+     Gamma |- t \in T.
+Proof.
+  intros Gamma t T.
+  eapply weakening.
+  discriminate.
+Qed.
+
+Lemma substitution_preserves_typing : forall Gamma x U t v T,
+  (x |-> U ; Gamma) |- t \in T ->
+  empty |- v \in U ->
+  Gamma |- [x:=v]t \in T.
+Proof with eauto.
+  intros Gamma x U t v T Ht Hv.
+  generalize dependent Gamma. generalize dependent T.
+  induction t; intros T Gamma H;
+  (* in each case, we'll want to get at the derivation of H *)
+    inversion H; clear H; subst; simpl; eauto.
+  - (* var *)
+    rename s into y. destruct (eqb_stringP x y); subst.
+    + (* x=y *)
+      rewrite update_eq in H2.
+      injection H2 as H2; subst.
+      apply weakening_empty. assumption.
+    + (* x<>y *)
+      apply T_Var. rewrite update_neq in H2; auto.
+  - (* abs *)
+    rename s into y, t into S.
+    destruct (eqb_stringP x y); subst; apply T_Abs.
+    + (* x=y *)
+      rewrite update_shadow in H5. assumption.
+    + (* x<>y *)
+      apply IHt.
+      rewrite update_permute; auto.
+Qed.
+
+
+Theorem preservation : forall t t' T,
+   empty |- t \in T ->
+   t --> t' ->
+   empty |- t' \in T.
+Proof with eauto.
+  intros t t' T HT. generalize dependent t'.
+  remember empty as Gamma.
+  induction HT;
+    intros t' HE; subst; inversion HE; subst...
+  - (* T_App *)
+    inversion HE; subst...
+    + (* ST_AppAbs *)
+      apply substitution_preserves_typing with T2...
+      inversion HT1...
+  - (* T_Fst *)
+    inversion HT...
+  - (* T_Snd *)
+    inversion HT...
+Qed.
+
+Inductive appears_free_in : string -> tm -> Prop :=
+  | afi_var : forall (x : string),
+      appears_free_in x <{ x }>
+  | afi_app1 : forall x t1 t2,
+      appears_free_in x t1 -> appears_free_in x <{ t1 t2 }>
+  | afi_app2 : forall x t1 t2,
+      appears_free_in x t2 -> appears_free_in x <{ t1 t2 }>
+  | afi_abs : forall x y T11 t12,
+        y <> x ->
+        appears_free_in x t12 ->
+        appears_free_in x <{ \y : T11, t12 }>
+  (* booleans *)
+  | afi_test0 : forall x t0 t1 t2,
+      appears_free_in x t0 ->
+      appears_free_in x <{ if t0 then t1 else t2 }>
+  | afi_test1 : forall x t0 t1 t2,
+      appears_free_in x t1 ->
+      appears_free_in x <{ if t0 then t1 else t2 }>
+  | afi_test2 : forall x t0 t1 t2,
+      appears_free_in x t2 ->
+      appears_free_in x <{ if t0 then t1 else t2 }>
+  (* pairs *)
+  | afi_pair1 : forall x t1 t2,
+      appears_free_in x t1 ->
+      appears_free_in x <{ (t1, t2) }>
+  | afi_pair2 : forall x t1 t2,
+      appears_free_in x t2 ->
+      appears_free_in x <{ (t1 , t2) }>
+  | afi_fst : forall x t,
+      appears_free_in x t ->
+      appears_free_in x <{ t.fst }>
+  | afi_snd : forall x t,
+      appears_free_in x t ->
+      appears_free_in x <{ t.snd }>.
+Hint Constructors appears_free_in : core.
+
+
+Definition closed (t:tm) :=  forall x, ~ appears_free_in x t.
+
+Lemma context_invariance : forall Gamma Gamma' t S,
+     Gamma |- t \in S ->
+     (forall x, appears_free_in x t -> Gamma x = Gamma' x) ->
+     Gamma' |- t \in S.
+Proof.
+  intros.
+  generalize dependent Gamma'.
+  induction H; intros; eauto 12.
+  - (* T_Var *)
+    apply T_Var. rewrite <- H0; auto.
+  - (* T_Abs *)
+    apply T_Abs.
+    apply IHhas_type. intros x1 Hafi.
+    (* the only tricky step... *)
+    destruct (eqb_stringP x x1); subst.
+    + rewrite update_eq.
+      rewrite update_eq.
+      reflexivity.
+    + rewrite update_neq; [| assumption].
+      rewrite update_neq; [| assumption].
+      auto.
+Qed.
+
+Lemma free_in_context : forall x t T Gamma,
+   appears_free_in x t ->
+   Gamma |- t \in T ->
+   exists T', Gamma x = Some T'.
+Proof with eauto.
+  intros x t T Gamma Hafi Htyp.
+  induction Htyp; inversion Hafi; subst...
+  - (* T_Abs *)
+    destruct IHHtyp as [T' Hctx]... exists T'.
+    unfold update, t_update in Hctx.
+    rewrite false_eqb_string in Hctx...
+Qed.
+
+Corollary typable_empty__closed : forall t T,
+    empty |- t \in T ->
+    closed t.
+Proof.
+  intros. unfold closed. intros x H1.
+  destruct (free_in_context _ _ _ _ H1 H) as [T' C].
+  discriminate C. Qed.
+
+Lemma step_deterministic :   deterministic step.
+Proof with eauto.
+   unfold deterministic.
+   intros t t' t'' E1 E2.
+   generalize dependent t''.
+   induction E1; intros t'' E2; inversion E2; subst; clear E2...
+  (* ST_AppAbs *)
+   - inversion H3.
+   - exfalso; apply value__normal in H...
+   (* ST_App1 *)
+   - inversion E1.
+   - f_equal...
+   - exfalso; apply value__normal in H1...
+   (* ST_App2 *)
+   - exfalso; apply value__normal in H3...
+   - exfalso; apply value__normal in H...
+   - f_equal...
+   - (* ST_IfTrue *)
+       inversion H3.
+   - (* ST_IfFalse *)
+       inversion H3.
+   (* ST_If *)
+   - inversion E1.
+   - inversion E1.
+   - f_equal...
+   (* ST_Pair1 *)
+   - f_equal...
+   - exfalso; apply value__normal in H1...
+   (* ST_Pair2 *)
+   - exfalso; apply value__normal in H...
+   - f_equal...
+   (* ST_Fst1 *)
+   - f_equal...
+   - exfalso.
+     inversion E1; subst.
+     + apply value__normal in H0...
+     + apply value__normal in H1...
+   (* ST_FstPair *)
+   - exfalso.
+     inversion H2; subst.
+     + apply value__normal in H...
+     + apply value__normal in H0...
+   (* ST_Snd1 *)
+   - f_equal...
+   - exfalso.
+     inversion E1; subst.
+     + apply value__normal in H0...
+     + apply value__normal in H1...
+   (* ST_SndPair *)
+   - exfalso.
+     inversion H2; subst.
+     + apply value__normal in H...
+     + apply value__normal in H0...
+Qed.
+
+
+Definition halts (t:tm) : Prop := exists t', t -->* t' /\ value t'.
+
+Lemma value_halts : forall v, value v -> halts v.
+Proof.
+  intros v H. unfold halts.
+  exists v. split.
+  - apply multi_refl.
+  - assumption.
+Qed.
+
+(*
+  Inductive R : ty -> tm -> Prop :=
+      | R_bool : forall b t, 
+                      empty |- t \in Bool ->
+                      halts t ->
+                      R Bool t
+      | R_arrow : forall T1 T2 t, 
+                      empty |- t \in (Arrow T1 T2) ->
+                      halts t ->
+                      (forall s, R T1 s -> R T2 (app t s)) ->
+                      R (Arrow T1 T2) t.
+*)
+
+Fixpoint R (T:ty) (t:tm) : Prop :=
+  empty |- t \in T /\ halts t /\
+  (match T with
+   | <{ Bool }> => True
+   | <{ T1 -> T2 }> => (forall s, R T1 s -> R T2 <{t s}> )
+   | <{ T1 * T2 }> => True
+   end).
+
+Lemma R_halts : forall {T} {t}, R T t -> halts t.
+Proof.
+  intros.
+  destruct T; unfold R in H; destruct H as [_ [H _]]; assumption.
+Qed.
+
+
+Lemma R_typable_empty : forall {T} {t}, R T t -> empty |- t \in T.
+Proof.
+  intros.
+  destruct T; unfold R in H; destruct H as [H _]; assumption.
+Qed.
+
+
+Lemma step_preserves_halting :
+  forall t t', (t --> t') -> (halts t <-> halts t').
+Proof.
+ intros t t' ST. unfold halts.
+ split.
+ - (* -> *)
+  intros [t'' [STM V]].
+  destruct STM.
+   + exfalso; apply value__normal in V; eauto.
+   + rewrite (step_deterministic _ _ _ ST H). exists z. split; assumption.
+ - (* <- *)
+  intros [t'0 [STM V]].
+  exists t'0. split; eauto.
+Qed.
+
+Lemma step_preserves_R : forall T t t', (t --> t') -> (R T t -> R T t').
+Proof.
+ induction T; intros t t' E Rt; unfold R; fold R; unfold R in Rt; fold R in Rt;
+               destruct Rt as [typable_empty_t [halts_t RRt]].
+  (* Bool *)
+  - split. eapply preservation; eauto.
+    split. apply (step_preserves_halting _ _ E); eauto.
+    auto.
+  (* Arrow *)
+  - split. eapply preservation; eauto.
+    split. apply (step_preserves_halting _ _ E); eauto.
+    intros.
+    eapply IHT2.
+    apply ST_App1. apply E.
+    apply RRt; auto.
+  - (* Pair *)
+    split. eapply preservation; eauto.
+    split. apply (step_preserves_halting _ _ E); eauto.
+    auto. (* Probably incorrect *)
+Qed.
+
+Lemma multistep_preserves_R : forall T t t',
+  (t -->* t') -> (R T t -> R T t').
+Proof.
+  intros T t t' STM; induction STM; intros.
+  assumption.
+  apply IHSTM. eapply step_preserves_R. apply H. assumption.
+Qed.
+
+Lemma step_preserves_R' : forall T t t',
+  empty |- t \in T -> (t --> t') -> R T t' -> R T t.
+Proof.
+  intros T. induction T; intros t t' Ht Hp Rt'; unfold R in Rt'; unfold R.
+  - destruct Rt' as [Ht' [Hhaltt' _]].
+    split. assumption.
+    split. rewrite (step_preserves_halting t t' Hp). assumption.
+    auto.
+  - fold R. fold R in Rt'.
+    destruct Rt' as [Ht' [Hhaltt' Hf]].
+    split. apply Ht.
+    split. rewrite (step_preserves_halting t t' Hp). assumption.
+    intros s Rs.
+    apply IHT2 with <{ t' s }>.
+    + eapply T_App. apply Ht. apply (R_typable_empty Rs).
+    + constructor. assumption.
+    + apply Hf. assumption.
+  - destruct Rt' as [Ht' [Hhaltt' _]].
+    split. assumption.
+    split. rewrite (step_preserves_halting t t' Hp). assumption.
+    auto.
+Qed.
+
+Lemma multistep_preserves_R' : forall T t t',
+  empty |- t \in T -> (t -->* t') -> (R T t' -> R T t).
+Proof.
+  intros T t t' HT STM.
+  induction STM; intros.
+    assumption.
+    eapply step_preserves_R'. assumption. apply H. apply IHSTM.
+    eapply preservation; eauto. auto.
+Qed.
+
+
+
+Definition env := list (string * tm).
+
+Fixpoint msubst (ss: env) (t: tm) : tm :=
+  match ss with
+  | nil           => t
+  | ((x, s)::ss') => msubst ss' <{ [x:=s]t }>
+  end.
+
+
+Definition tass := list (string * ty).
+
+Fixpoint mupdate (Gamma: context) (xts: tass) :=
+  match xts with
+  | nil             => Gamma
+  | ((x, v)::xts')  => update (mupdate Gamma xts') x v
+  end.
+
+
+Fixpoint lookup {X:Set} (k: string) (l: list (string * X)) : option X :=
+  match l with
+    | nil           => None
+    | (j, x) :: l'  =>
+      if eqb_string j k then Some x else lookup k l'
+  end.
+
+Fixpoint drop {X:Set} (n: string) (nxs: list (string * X)) : list (string * X) :=
+  match nxs with
+    | nil             => nil
+    | ((n', x)::nxs') =>
+        if eqb_string n' n 
+        then drop n nxs'
+        else (n', x) :: (drop n nxs')
+  end.
+
+
+Inductive instantiation : tass -> env -> Prop :=
+| V_nil :
+    instantiation nil nil
+| V_cons : forall x T v c e,
+    value v  ->  R T v ->
+    instantiation c e ->
+    instantiation ((x,T)::c) ((x,v)::e).
+
+
+Lemma vacuous_substitution : forall t x,
+     ~(appears_free_in x t) ->
+     forall t', <{ [x:=t']t }> = t.
+Proof with eauto.
+  intros t.
+  induction t; intros x Hnot_app t'.
+  - unfold subst.
+    unfold eqb_string.
+    destruct (string_dec x s) as [H | H]; subst.
+    + exfalso. apply Hnot_app...
+    + reflexivity.
+  - simpl.
+    assert (G2: ~ appears_free_in x t2). { intro H. apply Hnot_app. apply afi_app2. assumption. }
+    assert (G1: ~ appears_free_in x t1). { intro H. apply Hnot_app. apply afi_app1. assumption. }
+    rewrite (IHt1 x G1).
+    rewrite (IHt2 x G2).
+    reflexivity.
+  - simpl.
+    unfold eqb_string.
+    destruct (string_dec x s) as [H | H]; subst.
+    + reflexivity.
+    + assert (G: ~ appears_free_in x t0). { intro H'. apply Hnot_app. apply afi_abs... }
+      rewrite (IHt x G)...
+  - simpl...
+  - simpl...
+  - simpl.
+    assert (G: ~ appears_free_in x t1). { intro H'. apply Hnot_app. apply afi_test0... }
+    assert (G1: ~ appears_free_in x t2). { intro H'. apply Hnot_app. apply afi_test1... }
+    assert (G2: ~ appears_free_in x t3). { intro H'. apply Hnot_app. apply afi_test2... }
+    rewrite (IHt1 x G).
+    rewrite (IHt2 x G1).
+    rewrite (IHt3 x G2).
+    reflexivity.
+  - simpl.
+    assert (G1: ~ appears_free_in x t1). { intro H'. apply Hnot_app. apply afi_pair1... }
+    assert (G2: ~ appears_free_in x t2). { intro H'. apply Hnot_app. apply afi_pair2... }
+    rewrite (IHt1 x G1).
+    rewrite (IHt2 x G2).
+    reflexivity.
+  - simpl.
+    assert (G: ~ appears_free_in x t). { intro H'. apply Hnot_app. apply afi_fst... }
+    rewrite (IHt x G)...
+  - simpl.
+    assert (G: ~ appears_free_in x t). { intro H'. apply Hnot_app. apply afi_snd... }
+    rewrite (IHt x G)...
+Qed.
+
+
+Lemma subst_closed: forall t,
+     closed t -> forall x t', <{ [x:=t']t }> = t.
+Proof.
+  intros. apply vacuous_substitution. apply H. Qed.
+
+Lemma subst_not_afi : forall t x v,
+    closed v  ->  ~ appears_free_in x <{ [x:=v]t }>.
+Proof with eauto. (* rather slow this way *)
+  unfold closed, not.
+  induction t; intros x v P A; simpl in A.
+    - (* var *)
+     destruct (eqb_stringP x s)...
+     inversion A; subst. auto.
+    - (* app *)
+     inversion A; subst...
+    - (* abs *)
+     destruct (eqb_stringP x s)...
+     + inversion A; subst...
+     + inversion A; subst...
+    - (* tru *)
+     inversion A.
+    - (* fls *)
+     inversion A.
+    - (* test *)
+     inversion A; subst...
+    - (* pair *)
+     inversion A; subst...
+    - (* fst *)
+     inversion A; subst...
+    - (* snd *)
+     inversion A; subst...
+Qed.
+
+Lemma duplicate_subst : forall t' x t v,
+  closed v  ->  <{ [x:=t]([x:=v]t') }> = <{ [x:=v]t' }>.
+Proof.
+  intros. eapply vacuous_substitution. apply subst_not_afi. assumption.
+Qed.
+
+Lemma swap_subst : forall t x x1 v v1,
+    x <> x1 ->
+    closed v -> closed v1 ->
+    <{ [x1:=v1]([x:=v]t) }> = <{ [x:=v]([x1:=v1]t) }>.
+Proof with eauto.
+ induction t; intros; simpl.
+  - (* var *)
+   destruct (eqb_stringP x s); destruct (eqb_stringP x1 s).
+   + subst. exfalso...
+   + subst. simpl. rewrite <- eqb_string_refl. apply subst_closed...
+   + subst. simpl. rewrite <- eqb_string_refl. rewrite subst_closed...
+   + simpl. rewrite false_eqb_string... rewrite false_eqb_string...
+  - (* app *)
+    rewrite IHt1...
+    rewrite IHt2...
+  - (* abs *)
+    destruct (eqb_stringP x s); destruct (eqb_stringP x1 s).
+    + subst. simpl. rewrite <- eqb_string_refl...
+    + subst. simpl. rewrite false_eqb_string... rewrite <- eqb_string_refl...
+    + subst. simpl. rewrite <- eqb_string_refl... rewrite false_eqb_string...
+    + subst. simpl. rewrite false_eqb_string... rewrite false_eqb_string...
+      rewrite IHt...
+  - reflexivity.
+  - reflexivity.
+  - rewrite IHt1...
+    rewrite IHt2...
+    rewrite IHt3...
+  - rewrite IHt1...
+    rewrite IHt2...
+  - rewrite IHt...
+  - rewrite IHt...
+Qed.
+
+
+
+
+Lemma msubst_closed: forall t, closed t  ->  forall ss, msubst ss t = t.
+Proof.
+  induction ss.
+    reflexivity.
+    destruct a. simpl. rewrite subst_closed; assumption.
+Qed.
+
+Fixpoint closed_env (env:env): Prop :=
+  match env with
+  | nil         => True
+  | (x,t)::env' => closed t /\ closed_env env'
+  end.
+
+Lemma subst_msubst: forall env x v t, closed v  ->  closed_env env ->
+    msubst env <{ [x:=v]t }> = <{ [x:=v] { msubst (drop x env) t } }> .
+Proof.
+  induction env0; intros; auto.
+  destruct a. simpl.
+  inversion H0.
+  destruct (eqb_stringP s x).
+  - subst. rewrite duplicate_subst; auto.
+  - simpl. rewrite swap_subst; eauto.
+Qed.
+
+Lemma msubst_var: forall ss x, closed_env ss ->
+   msubst ss (tm_var x) =
+   match lookup x ss with
+   | Some t => t
+   | None   => tm_var x
+  end.
+Proof.
+  induction ss; intros.
+    reflexivity.
+    destruct a.
+     simpl. destruct (eqb_string s x).
+      apply msubst_closed. inversion H; auto.
+      apply IHss. inversion H; auto.
+Qed.
+
+Lemma msubst_abs: forall ss x T t,
+  msubst ss <{ \ x : T, t }> = <{ \x : T, {msubst (drop x ss) t} }>.
+Proof.
+  induction ss; intros.
+    reflexivity.
+    destruct a.
+      simpl. destruct (eqb_string s x); simpl; auto.
+Qed.
+
+Lemma msubst_app : forall ss t1 t2,
+    msubst ss <{ t1 t2 }> = <{ {msubst ss t1} ({msubst ss t2}) }>.
+Proof.
+ induction ss; intros.
+   reflexivity.
+   destruct a.
+    simpl. rewrite <- IHss. auto.
+Qed.
+
+Lemma msubst_true : forall ss,
+    msubst ss <{ true }> = <{ true }>.
+Proof.
+ induction ss; intros.
+ - reflexivity.
+ - simpl. rewrite IHss.
+   destruct a. reflexivity.
+Qed.
+
+Lemma msubst_false : forall ss,
+    msubst ss <{ false }> = <{ false }>.
+Proof.
+ induction ss; intros.
+ - reflexivity.
+ - simpl. rewrite IHss.
+   destruct a. reflexivity.
+Qed.
+
+Lemma mupdate_lookup : forall (c : tass) (x:string),
+    lookup x c = (mupdate empty c) x.
+Proof.
+  induction c; intros.
+    auto.
+    destruct a. unfold lookup, mupdate, update, t_update. destruct (eqb_string s x); auto.
+Qed.
+
+Lemma mupdate_drop : forall (c: tass) Gamma x x',
+      mupdate Gamma (drop x c) x'
+        = if eqb_string x x' then Gamma x' else mupdate Gamma c x'.
+Proof.
+  induction c; intros.
+  - destruct (eqb_stringP x x'); auto.
+  - destruct a. simpl.
+    destruct (eqb_stringP s x).
+    + subst. rewrite IHc.
+      unfold update, t_update. destruct (eqb_stringP x x'); auto.
+    + simpl. unfold update, t_update. destruct (eqb_stringP s x'); auto.
+      subst. rewrite false_eqb_string; congruence.
+Qed.
+
+
+Lemma instantiation_domains_match: forall {c} {e},
+    instantiation c e ->
+    forall {x} {T},
+      lookup x c = Some T -> exists t, lookup x e = Some t.
+Proof.
+  intros c e V. induction V; intros x0 T0 C.
+    solve_by_invert.
+    simpl in *.
+    destruct (eqb_string x x0); eauto.
+Qed.
+
+Lemma instantiation_env_closed : forall c e,
+  instantiation c e -> closed_env e.
+Proof.
+  intros c e V; induction V; intros.
+    econstructor.
+    unfold closed_env. fold closed_env.
+    split; [|assumption].
+    eapply typable_empty__closed. eapply R_typable_empty. eauto.
+Qed.
+
+Lemma instantiation_R : forall c e,
+    instantiation c e ->
+    forall x t T,
+      lookup x c = Some T ->
+      lookup x e = Some t -> R T t.
+Proof.
+  intros c e V. induction V; intros x' t' T' G E.
+    solve_by_invert.
+    unfold lookup in *. destruct (eqb_string x x').
+      inversion G; inversion E; subst. auto.
+      eauto.
+Qed.
+
+Lemma instantiation_drop : forall c env,
+    instantiation c env ->
+    forall x, instantiation (drop x c) (drop x env).
+Proof.
+  intros c e V. induction V.
+    intros. simpl. constructor.
+    intros. unfold drop.
+    destruct (eqb_string x x0); auto. constructor; eauto.
+Qed.
+
+
+Lemma multistep_App2 : forall v t t',
+  value v -> 
+  (t -->* t') -> 
+  <{ v t }> -->* <{ v t' }>.
+Proof.
+  intros v t t' V STM. induction STM.
+   apply multi_refl.
+   eapply multi_step.
+     apply ST_App2; eauto. auto.
+Qed.
+
+
+
+ Lemma msubst_preserves_typing : forall c e,
+     instantiation c e ->
+     forall Gamma t S, (mupdate Gamma c) |- t \in S ->
+     Gamma |- { (msubst e t) } \in S.
+Proof.
+  induction 1; intros.
+    simpl in H. simpl. auto.
+    simpl in H2. simpl.
+    apply IHinstantiation.
+    eapply substitution_preserves_typing; eauto.
+    apply (R_typable_empty H0).
+Qed.
+
+
+Lemma msubst_R : forall c env t T,
+    (mupdate empty c) |- t \in T ->
+    instantiation c env ->
+    R T (msubst env t).
+Proof.
+  intros c env0 t T HT V.
+  generalize dependent env0.
+  (* We need to generalize the hypothesis a bit before setting up the induction. *)
+  remember (mupdate empty c) as Gamma.
+  assert (forall x, Gamma x = lookup x c). {
+    intros. rewrite HeqGamma. rewrite mupdate_lookup. auto. }
+  clear HeqGamma.
+  generalize dependent c.
+  induction HT; intros.
+  - (* T_Var *)
+   rewrite H0 in H. destruct (instantiation_domains_match V H) as [t P].
+   eapply instantiation_R; eauto.
+   rewrite msubst_var. rewrite P. auto. eapply instantiation_env_closed; eauto.
+  - (* T_Abs *)
+    rewrite msubst_abs.
+    (* We'll need variants of the following fact several times, so its simplest to
+       establish it just once. *)
+    assert (WT : empty |- \x : T2, {msubst (drop x env0) t1 } \in (T2 -> T1) ).
+    { eapply T_Abs. eapply msubst_preserves_typing.
+      { eapply instantiation_drop; eauto. }
+      eapply context_invariance.
+      { apply HT. }
+      intros.
+      unfold update, t_update. rewrite mupdate_drop. destruct (eqb_stringP x x0).
+      + auto.
+      + rewrite H.
+        clear - c n. induction c.
+        simpl. rewrite false_eqb_string; auto.
+        simpl. destruct a. unfold update, t_update.
+        destruct (eqb_string s x0); auto. }
+    unfold R. fold R. split.
+       auto.
+     split. apply value_halts. apply v_abs.
+     intros.
+     destruct (R_halts H0) as [v [P Q]].
+     pose proof (multistep_preserves_R _ _ _ P H0).
+     apply multistep_preserves_R' with (msubst ((x,v)::env0) t1).
+       eapply T_App. eauto.
+       apply R_typable_empty; auto.
+       eapply multi_trans. eapply multistep_App2; eauto.
+       eapply multi_R.
+       simpl. rewrite subst_msubst.
+       eapply ST_AppAbs; eauto.
+       eapply typable_empty__closed.
+       apply (R_typable_empty H1).
+       eapply instantiation_env_closed; eauto.
+       eapply (IHHT ((x,T2)::c)).
+          intros. unfold update, t_update, lookup. destruct (eqb_string x x0); auto.
+       constructor; auto.
+  - (* T_App *)
+    rewrite msubst_app.
+    destruct (IHHT1 c H env0 V) as [_ [_ P1]].
+    pose proof (IHHT2 c H env0 V) as P2. fold R in P1. auto.
+  - (* true *) simpl. auto.
+    rewrite msubst_true.
+    split. constructor.
+    split. unfold halts. exists <{ true }>. auto.
+    auto.
+  - (* false *) simpl. auto.
+    rewrite msubst_false.
+    split. constructor.
+    split. unfold halts. exists <{ false }>. auto.
+    auto.
+  - (* if *)
+    simpl.
+  (* TODO *) Admitted.
+
+Theorem normalization : forall t T, empty |- t \in T  ->  halts t.
+Proof.
+  intros.
+  replace t with (msubst nil t) by reflexivity.
+  apply (@R_halts T).
+  apply (msubst_R nil); eauto.
+  eapply V_nil.
+Qed.
+
